
\section{Ολοκληρώματα}

\subsection{Ορισμός Αόριστου Ολοκληρώματος}

\[
  \int f(x)\, dx = F(x) + c \Leftrightarrow F'(x) = f(x)
\]

\subsection{Ολοκληρώματα Βασικών Συναρτήσεων}

\begin{tabular}{@{}*{2}{>{$}l<{$}}@{}}
  \int 0 \,dx = c \\
  \int 1 \,dx = \int \,dx = x  \\
  \int x^{n} \,dx = \frac{x^{n+1}}{n+1}, \qq{$n\neq -1$} \\
  \int \frac{1}{x} \,dx = \ln\abs{x}  \\
  \int a^{x} \,dx = \frac{a^{x}}{\ln a}, \qq{$a>0$, $a\neq 1$} \\
  \int e^{x} \,dx = e^{x}  \\
  \int \sqrt[n]{x^{m}} \,dx =  \int x^{\frac{m}{n}} \,dx = \frac{x^{\frac{m}{n}+1}}{\frac{m}{n}+1} \\
  \int \sin x \,dx = -\cos x & \int \sinh x \,dx = \cosh x \\
  \int \cos x \,dx = \sin x & \int \cosh x \,dx = \sinh x \\
  \int \tan x \,dx = \ln\sec x = -\ln\cos x & \int \tanh x \,dx = \ln\cosh x \\
  \int \cot x \,dx = \ln\sin x & \int \coth x \,dx = \ln\sinh x \\
  \int \sec x \,dx = \ln(\sec x + \tan x) = \ln\tan(\frac{x}{2}+\frac{\pi}{4}) & \int \sech x \,dx = \sin^{-1}(\tanh x) \\
  \int \csc x \,dx = \ln(\csc x - \cot x) = \ln\tan\frac{x}{2} & \int \csch x \,dx = \ln\tanh\frac{x}{2} \\
  \int \sec^{2}x \,dx = \tan x & \int \sech^{2}x \,dx = \tanh x \\
  \int \csc^{2}x \,dx = -\cot x & \int \csch^{2}x \,dx = -\coth x \\
  \int \tan^{2}x \,dx = \tan x - x  & \int \tanh^{2}x \,dx = x - \tanh x \\
  \int \cot^{2}x \,dx = -\cot x - x & \int \coth^{2}x \,dx = x - \coth x \\
  \int \sin^{2}x \,dx = \frac{x}{2} - \frac{\sin 2x}{4} & \int \sinh^{2}x \,dx = \frac{\sinh 2x}{4}-\frac{x}{2} \\
  \int \cos^{2}x \,dx = \frac{x}{2} + \frac{\sin 2x}{4} & \int \cosh^{2}x \,dx = \frac{\sinh 2x}{4}+\frac{x}{2} \\
  \int \sec x \tan x \,dx = \sec x & \int \sech x \tanh x \,dx = -\sech x \\
  \int \csc x \cot x \,dx = -\csc x & \int \csch x \coth x \,dx = -\csch x
\end{tabular}

\begin{tabular}{@{}>{$}l<{$}@{}}
  \int \frac{1}{x^{2}+a^{2}} \,dx  = \frac{1}{a}\tan^{-1}\frac{x}{a} \\
  \int \frac{1}{x^{2}-a^{2}} \,dx  = \frac{1}{2a}\ln(\frac{x-a}{x+a}) = -\frac{1}{a}\cot^{-1}\frac{x}{a} \\
  \int \frac{1}{a^{2}-x^{2}} \,dx  = \frac{1}{2a}\ln(\frac{a+x}{a-x}) = \frac{1}{a}\tanh^{-1}\frac{x}{a}  \\
  \int \frac{1}{\sqrt{a^{2}-x^{2}}} \,dx  = \sin^{-1}\frac{x}{a} \\
  \int \frac{1}{\sqrt{x^{2}+a^{2}}} \,dx  = \ln(x+\sqrt{x^{2}+a^{2}}) = \sin^{-1}\frac{x}{a} \\
  \int \frac{1}{\sqrt{x^{2}-a^{2}}} \,dx  = \ln(x+\sqrt{x^{2}-a^{2}}) \\
  \int \frac{1}{x\sqrt{x^{2}-a^{2}}} \,dx = \frac{1}{a}\sec^{-1}\abs{\frac{x}{a}} \\
  \int \frac{1}{x\sqrt{x^{2}+a^{2}}} \,dx = -\frac{1}{a}\ln(\frac{a+\sqrt{x^{2}+a^{2}}}{x}) \\
  \int \frac{1}{x\sqrt{a^{2}-x^{2}}} \,dx = -\frac{1}{a}\ln(\frac{a+\sqrt{a^{2}-x^{2}}}{x})
\end{tabular}

\subsection{$ax+b$}

\begin{tabular}{@{}>{$}l<{$}@{}}
  \int \frac{dx}{ax+b} \,dx = \frac{1}{a}\ln(ax+b) \\
  \int \frac{x}{ax+b} \,dx = \frac{x}{a} - \frac{b}{a^{2}}\ln(ax+b) \\
  \int \frac{dx}{x(ax+b)} \,dx = \frac{1}{b}\ln(\frac{x}{ax+b}) \\
  \int \frac{1}{(ax+b)^{2}}\, dx = \frac{-1}{a(ax+b)} \\
  \int \frac{x}{(ax+b)^{2}}\, dx = \frac{b}{a^{2}(ax+b)}+\frac{1}{a^{2}}\ln(ax+b) \\
  \int \frac{1}{x(ax+b)^{2}} \,dx = \frac{1}{b^{2}}\ln(\frac{x}{ax+b}) \\
  \int (ax+b)^{n} \,dx = \frac{(ax+b)^{n+1}}{a(n+1)}, n\neq -1 \\
  \int x(ax+b)^{n} \,dx = \frac{(ax+b)^{n+2}}{a^{2}(n+2)} - \frac{b(ax+b)^{n+1}}{a^{2}(n+1)}, n\neq -1, -2 \\
  \int {x^{m}}(ax+b)^{n} \,dx = \begin{cases}
  \frac{x^{m+1}(ax+b)^{n}}{m+n+1} + \frac{nb}{m+n+1}\int x^{m}(ax+b)^{n-1}\,dx \\
  \frac{x^{m}(ax+b)^{n+1}}{a(m+n+1)} - \frac{mb}{a(m+n+1)}\int x^{m-1}(ax+b)^n \,dx \\
  \frac{-x^{m+1}(ax+b)^{n+1}}{b(n+1)} + \frac{m+n+2}{b(n+1)}\int x^{m}(ax+b)^{n+1}\,dx
\end{cases}
\end{tabular}

\subsection{$\sqrt{ax+b}$}

\begin{tabular}{@{}>{$}l<{$}@{}}
  \int \frac{dx}{\sqrt{ax+b}} \,dx = \frac{2\sqrt{ax+b}}{a} \\
  \int \frac{xdx}{\sqrt{ax+b}} \,dx = \frac{2(ax-2b)}{3a^{2}}\sqrt{ax+b} \\
  \int \frac{dx}{x\sqrt{ax+b}} \,dx =
    \begin{cases}
      \frac{1}{\sqrt{b}}\ln(\frac{\sqrt{ax+b}-\sqrt{b}}{\sqrt{ax+b}+\sqrt{b}}) \\
      \frac{2}{\sqrt{-b}}\tan^{-1}\sqrt{\frac{ax+b}{-b}}
    \end{cases} \\
  \int \sqrt{ax+b} \,dx = \frac{2\sqrt{(ax+b)^{3}}}{3a} \\
  \int x\sqrt{ax+b} \,dx = \frac{2(3ax-2b)}{15a^{2}}\sqrt{(ax+b)^{3}} \\
  \int \frac{\sqrt{ax+b}}{x} \,dx = 2\sqrt{ax+b} +b\int\frac{dx}{x\sqrt{ax+b}} \\
  \int\frac{x^{m}}{\sqrt{ax+b}} \,dx = \frac{2x^{m}\sqrt{ax+b}}{a(2m+1)} - \frac{2mb}{a(2m+1)}\int \frac{x^{m-1}}{\sqrt{ax+b}} \,dx \\
  \int \frac{dx}{x^{m}\sqrt{ax+b}} \,dx = -\frac{\sqrt{ax+b}}{b(m-1)x^{m-1}}-\frac{a(2m-3)}{b(2m-2)}  \int \frac{dx}{x^{m-1}\sqrt{ax+b}} \\
  \int x^{m}\sqrt{ax+b} \,dx = \frac{2x^{m}}{a(2m+3)}(ax+b)^{frac{3}{2}}-\frac{2mb}{a(2m+3)}\int x^{m-1}\sqrt{ax+b} \,dx \\
  \int \frac{\sqrt{ax+b}}{x^{m}} \,dx = -\frac{\sqrt{ax+b}}{(m-1)x^{m-1}} + \frac{a}{2(m-1)}\int \frac{dx}{x^{m-1}\sqrt{ax+b}}\, dx \\
  \int \frac{\sqrt{ax+b}}{x^{m}} \,dx = -\frac{(ax+b)^{\frac{3}{2}}}{b(m-1)x^{m-1}} - \frac{a(2m-5)}{b(2m-2)}\int \frac{\sqrt{ax+b}}{x^{m-1}} \,dx \\
  \int (ax+b)^{\frac{3}{2}} \,dx = \frac{2(ax+b)^{\frac{(m+2)}{2}}}{a^{2}(m+2)} \,dx \\\
  \int x(ax+b)^{\frac{m}{2}} \,dx = \frac{2(ax+b)^{\frac{m+4}{2}}}{a^{2}(m+4)} - \frac{2b(ax+b)^{\frac{m+2}{2}}}{a^{2}(m+2)} \\
  \int \frac{(ax+b)^{\frac{m}{2}}}{x} \,dx = \frac{2(ax+b)^{\frac{m}{2}}}{m}+b\int \frac{(ax+b)^{\frac{m-2}{2}}}{x} \,dx \\
  \int \frac{dx}{x(ax+b)^{\frac{m}{2}}} \,dx = \frac{2}{b(m-2)(ax+b)^{\frac{m-2}{2}}} + \frac{1}{b}\int \frac{dx}{x(ax+b)^{\frac{m-2}{2}}} \,dx
\end{tabular}

\subsection{$(ax+b), (px+q)$}


\begin{tabular}{@{}>{$}l<{$}@{}}
  \int \frac{dx}{(ax+b)(px+q)} = \frac{1}{bp-aq}\ln(\frac{px+q}{ax+b}) \\
  \int \frac{x}{(ax+b)(px+q)} \,dx = \frac{1}{bp-aq}\{\frac{b}{a}\ln(ax+b)-\frac{q}{p}\ln(px+q)\} \\
  \int \frac{1}{(ax+b)^{2}(px+q)} \,dx = \frac{1}{bp-aq}\{\frac{1}{ax+b}+\frac{p}{bp-aq}\ln(\frac{px+q}{ax+b})\} \\
  \int \frac{x}{(ax+b)^{2}(px+q)} \,dx = \frac{1}{bp-aq}\{\frac{q}{bp-aq}\ln(\frac{ax+b}{px+q})-\frac{b}{a(ax+b)}\} \\
  \int \frac{1}{(ax+b)^{m}(px+q)^{n}} \,dx = \frac{-1}{(n-1)(bp-aq)}\{\frac{1}{(ax+b)^{m-1}(px+q)^{n-1}}+a(m+n-2)\int \frac{(ax+b)^{m}}{(px+q)^{n-1}} \,dx\} \\
  \int\frac{ax+b}{px+q} \,dx = \frac{ax}{p}+\frac{bp-aq}{p^{2}}\ln(px+q) \\
  \int \frac{(ax+b)^{m}}{(px+q)^{n}} \,dx =
    \begin{cases}
      \frac{-1}{(n-1)(bp-aq)}\{\frac{(ax+b)^{m+1}}{(px+q)^{n-1}}+a(n-m-2)\int \frac{(ax+b)^{m}}{(px+q)^{n-1}}\,dx \} \\
      \frac{-1}{p(n-m-1)}\{\frac{(ax+b)^{m}}{(px+q)^{n-1}}+m(bp-aq)\int\frac{(ax+b)^{m-1}}{(px+q)^{n}} \,dx \} \\
      \frac{-1}{p(n-1)}\{\frac{(ax+b)^{m}}{(px+q)^{n-1}}-ma\int\frac{(ax+b)^{m-1}}{(px+q)^{n-1}}\, dx\}
    \end{cases}
\end{tabular}


\subsection{$\sqrt{ax+b}, px+q$}

\begin{tabular}{@{}>{$}l<{$}@{}}
  \int\frac{px+q}{\sqrt{ax+b}} \,dx = \frac{2(apx+3aq-2bp)}{3a^{2}}\sqrt{ax+b} \\
  \int\frac{1}{(px+q)\sqrt{ax+b}} =
  \begin{cases}
    \frac{1}{\sqrt{bp-aq}\sqrt{p}}\ln(\frac{\sqrt{p(ax+b)}-\sqrt{bp-aq}}{\sqrt{p(ax+b)}+\sqrt{bp-aq}}) \\
    \frac{2}{\sqrt{bp-aq}\sqrt{p}}\tan^{-1}\sqrt{\frac{p(ax+b)}{aq-bp}}
  \end{cases} \\
  \int\frac{\sqrt{ax+b}}{px+q} \,dx =
  \begin{cases}
     \frac{2\sqrt{ax+b}}{p}+\frac{\sqrt{bp-aq}}{p\sqrt{p}}\ln(\frac{\sqrt{p(ax+b)}-\sqrt{bp-aq}}{\sqrt{p(ax+b)}+\sqrt{bp-aq}}) \\
     \frac{2\sqrt{ax+b}}{p}-\frac{2\sqrt{bp-aq}}{p\sqrt{p}}\tan^{-1}\sqrt{\frac{p(ax+b)}{aq-bp}}
  \end{cases} \\
  \int(px+q)^{n}\sqrt{ax+b} \,dx = \frac{2(px+q)^{n+1}\sqrt{ax+b}}{p(2n+3)}+\frac{bp-aq}{p(2n+3)}\int\frac{dx}{(px+q)\sqrt{ax+b}} \,dx \\
  \int\frac{(px+q)^{n}}{\sqrt{ax+b}} \, dx = \frac{2(px+q)^{n}\sqrt{ax+b}}{a(2n+1)} + \frac{2n(aq-bp)}{a(2n+1)}\int\frac{(px+q)^{n-1}}{\sqrt{ax+b}} \,dx \\
  \int\frac{\sqrt{ax+b}}{(px+q)^{n}} \,dx = \frac{-\sqrt{ax+b}}{p(n-1)(px+q)^{n-1}} + \frac{a}{2p(n-1)}\int \frac{1}{(px+q)^{n-1}\sqrt{ax+b}} \,dx
\end{tabular}


\subsection{$\sqrt{ax+b}, \sqrt{px+q}$}

\begin{tabular}{@{}>{$}l<{$}@{}}
\int \frac{dx}{\sqrt{(ax+b)(px+q)}} \,dx =
  \begin{cases}
    \frac{2}{\sqrt{ap}}\ln(\sqrt{a(px+q)}+\sqrt{p(ax+b)}) \\
    \frac{2}{\sqrt{-ap}}\tan^{-1}\sqrt{\frac{-p(ax+b)}{a(px+q)}}
  \end{cases} \\
  \int \frac{x}{\sqrt{(ax+b)(px+q)}} \,dx = \frac{\sqrt{(ax+b)(px+q)}}{ap} - \frac{bp+aq}{2ap}\int\frac{dx}{\sqrt{(ax+b)(px+q)}} \\
  \int \sqrt{(ax+b)(px+q)} \,dx = \frac{2apx+bp+aq}{4ap}\sqrt{(ax+b)(px+q)}-\frac{(bp-aq)^{2}}{8ap}\int\frac{dx}{\sqrt{(ax+b)(px+q)}} \\
  \int\sqrt{\frac{px+q}{ax+b}} \,dx = \frac{\sqrt{(ax+b)(px+q)}}{a}+\frac{aq-bp}{2a}\int\frac{dx}{\sqrt{(ax+b)(px+q)}} \\
  \int\frac{dx}{(px+q)\sqrt{(ax+b)(px+q)}}=\frac{2\sqrt{ax+b}}{(aq-bp)\sqrt{px+q}}
\end{tabular}

\subsection{$x^{2}+a^{2}$}

\begin{tabular}{@{}>{$}l<{$}@{}}
  \int\frac{dx}{x^{2}+a^{2}} = \frac{1}{a}\tan^{-1}\frac{x}{a} \\
  \int\frac{x}{x^{2}+a^{2}} \,dx = \frac{1}{2}\ln(x^{2}+a^{2}) \\
  \int\frac{dx}{x(x^{2}+a^{2})} = \frac{1}{2a^{2}}\ln(\frac{x^{2}}{x^{2}+a^{2}}) \\
  \int\frac{dx}{(x^{2}+a^{2})^{2}} = \frac{x}{2a^{2}(x^{2}+a^{2})}+\frac{1}{2a^{3}}\tan^{-1}\frac{x}{a} \\
  \int\frac{x}{(x^{2}+a^{2})^{2}} \,dx = \frac{-1}{2(x^{2}+a^{2})^{2}} \\
  \int\frac{1}{x(x^{2}+a^{2})^{2}} \,dx = \frac{1}{2a^{2}(x^{2}+a^{2})}+\frac{1}{2a^{4}}\ln(\frac{x^{2}}{x^{2}+a^{2}}) \\
  \int\frac{1}{(x^{2}+a^{2})^{n}} = \frac{x}{2(n-1)a^{2}(x^{2}+a^{2})^{n-1}}+\frac{2n-3}{a^{2}(2n-2)}\int\frac{dx}{(x^{2}+a^{2})^{n-1}} \\
  \int\frac{x}{(x^{2}+a^{2})^{n}} \,dx = \frac{-1}{2(n-1)(x^{2}+a^{2})^{n-1}} \\
  \int\frac{dx}{x(x^{2}+a^{2})^{n}} \,dx = \frac{1}{2(n-1)a^{2}(x^{2}+a^{2})^{n-1}}+\frac{1}{a^{2}}\int\frac{dx}{x(x^{2}+a^{2})^{n-1}} \\
  \int{x^{m}}{(x^{2}+a^{2})^{n}} = \int\frac{x^{m-2}}{(x^{2}+a^{2})^{n-1}} - a^{2}\int\frac{x^{m-2}}{(x^{2}+a^{2})^{n}} \\
  \int\frac{1}{x^{m}(x^{2}+a^{2})^{n}} \,dx = \frac{1}{a^{2}}\int\frac{dx}{x^{m}(x^{2}+a^{2})^{n-1}} - \frac{1}{a^{2}}\int\frac{dx}{x^{m-2}(x^{2}+a^{2})^{n}}
\end{tabular}

\subsection{$x^{2}-a^{2}$}

\begin{tabular}{@{}>{$}l<{$}@{}}
  \int\frac{dx}{x^{2}-a^{2}} = \frac{1}{2a}\ln(\frac{x-a}{x+a}) = -\frac{1}{a}\coth^{-1}\frac{x}{a} \\
  \int\frac{x}{x^{2}-a^{2}} = \frac{1}{2}\ln(x^{2}-a^{2}) \\
  \int\frac{1}{x(x^{2}-a^{2})} \,dx = \frac{1}{2a^{2}}\ln(\frac{x^{2}-a^{2}}{x^{2}}) \\
  \int\frac{dx}{(x^{2}-a^{2})^{2}} \,dx = \frac{-x}{2a^{2}(x^{2}-a^{2})}-\frac{1}{4a^{3}}\ln(\frac{x-a}{x+a}) \\
  \int\frac{x}{(x^{2}-a^{2})^{2}} \,dx = \frac{-1}{2(x^{2}-a^{2})} \\
  \int\frac{1}{x(x^{2}-a^{2})^{2}} \,dx = \frac{-1}{2a^{2}(x^{2}-a^{2})} + \frac{1}{2a^{4}}\ln(\frac{x^{2}}{x^{2}-a^{2}}) \\
  \int\frac{dx}{(x^{2}-a^{2})^{n}} = \frac{-x}{2a^{2}(n-1)(x^{2}-a^{2})^{n-1}} - \frac{2n-3}{a^{2}(2n-2)}\int\frac{dx}{(x^{2}-a^{2})^{n-1}} \\
  \int\frac{x}{(x^{2}-a^{2})^{n}} \,dx = \frac{-1}{2(n-1)(x^{2}-a^{2})^{n-1}} \\
  \int\frac{1}{x(x^{2}-a^{2})^{n}} \,dx = \frac{-1}{2a^{2}(n-1)(x^{2}-a^{2})^{n-1}} - \frac{1}{a^{2}}\int\frac{dx}{x(x^{2}-a^{2})^{n-1}} \\
  \int\frac{x^{m}}{(x^{2}-a^{2})^{n}} \,dx = \frac{x^{m-2}}{(x^{2}-a^{2})^{n-1}} \,dx + a^{2}\int\frac{x^{m-2}}{x(x^{2}-a^{2})^{n-1}} \\
  \int\frac{dx}{x^{m}(x^{2}-a^{2})^{n}} = \frac{1}{a^{2}}\int\frac{dx}{x^{m-2}(x^{2}-a^{2})^{n}} - \frac{1}{a^{2}}\int\frac{dx}{x^{m}(x^{2}-a^{2})^{n-1}}
\end{tabular}

\subsection{$a^{2}-x^{2}$}

\begin{tabular}{@{}>{$}l<{$}@{}}
  \int\frac{dx}{a^{2}-x^{2}} = \frac{1}{2a}\ln(\frac{a+x}{a-x}) = \frac{1}{a}\tanh^{-1}\frac{x}{a} \\
  \int\frac{x}{a^{2}-x^{2}} \,dx = -\frac{1}{2}\ln(a^{2}-x^{2}) \\
  \int\frac{dx}{x(a^{2}-x^{2})} = \frac{1}{2a^{2}}\ln(\frac{x^{2}}{a^{2}-x^{2}}) \\
  \int\frac{dx}{(a^{2}-x^{2})^{2}} = \frac{x}{2a^{2}(a^{2}-x^{2})} + \frac{1}{4a^{3}}\ln(\frac{a+x}{a-x}) \\
  \int\frac{x}{(a^{2}-x^{2})^{2}} \,dx = \frac{1}{2(a^{2}-x^{2})} \\
  \int\frac{1}{x(a^{2}-x^{2})^{2}} \,dx = \frac{1}{2a^{2}(a^{2}-x^{2})} + \frac{1}{2a^{4}}\ln(\frac{x^{2}}{a^{2}-x^{2}}) \\
  \int\frac{dx}{(a^{2}-x^{2})^{n}} = \frac{x}{2a^{2}(n-1)(a^{2}-x^{2})^{n-1}}+\frac{2n-3}{a^{2}(2n-2)}\int\frac{dx}{(a^{2}-x^{2})^{n-1}} \\
  \int\frac{x}{(a^{2}-x^{2})^{n}} \,dx = \frac{1}{2(n-1)(a^{2}-x^{2})^{n-1}} \\
  \int\frac{dx}{x(a^{2}-x^{2})^{n}} = \frac{1}{2a^{2}(n-1)(a^{2}-x^{2})^{n-1}} + \frac{1}{a^{2}}\int\frac{dx}{x(a^{2}-x^{2})^{n-1}} \\
  \int\frac{x^{m}}{(a^{2}-x^{2})^{n}} \,dx = a^{2}\int\frac{x^{m-2}}{(a^{2}-x^{2})^{n}}\,dx - \int\frac{x^{m-2}}{(a^{2}-x^{2})^{n-1}} \\
  \int\frac{dx}{x^{m}(a^{2}-x^{2})^{n}} = \frac{1}{a^{2}}\int\frac{dx}{x^{m}(a^{2}-x^{2})^{n-1}} + \frac{1}{a^{2}}\int\frac{dx}{x^{m-2}(a^{2}-x^{2})^{n}}
\end{tabular}




\subsection{$\sqrt{x^{2}+a^{2}}$}

\begin{tabular}{@{}>{$}l<{$}@{}}
  \int\frac{1}{\sqrt{x^{2}+a^{2}}}\,dx = \ln(x+\sqrt{x^{2}+a^{2}}) = \sin^{-1}\frac{x}{a} \\
  \int\frac{x}{\sqrt{x^{2}+a^{2}}}\,dx = \sqrt{x^{2}+a^{2}} \\
  \int\frac{1}{x\sqrt{x^{2}+a^{2}}}\,dx = -\frac{1}{a}\ln(\frac{a+\sqrt{x^{2}+a^{2}}}{x}) \\
  \int\sqrt{x^{2}+a^{2}}\,dx = \frac{x\sqrt{x^{2}+a^{2}}}{2}+\frac{a^{2}}{2}\ln(x+\sqrt{x^{2}+a^{2}}) \\
  \int x\sqrt{x^{2}+a^{2}}\,dx = \frac{(x^{2}+a^{2})^{\frac{3}{2}}}{3} \\
  \int\frac{\sqrt{x^{2}+a^{2}}}{x}\,dx = \sqrt{x^{2}+a^{2}}-a\ln(\frac{a+\sqrt{x^{2}+a^{2}}}{x}) \\
\end{tabular}


\subsection{$\sqrt{x^{2}-a^{2}}$}

\begin{tabular}{@{}>{$}l<{$}@{}}
  \int\frac{1}{\sqrt{x^{2}-a^{2}}}\,dx = \ln(x+\sqrt{x^{2}-a^{2}}) \\
  \int\frac{x}{\sqrt{x^{2}-a^{2}}}\,dx = \frac{x\sqrt{x^{2}-a^{2}}}{2}+\frac{a^{2}}{2}\ln(x+\sqrt{x^{2}-a^{2}}) \\
  \int\frac{1}{x\sqrt{x^{2}-a^{2}}}\,dx = \frac{1}{a}\sec^{-1}\abs{\frac{x}{a}} \\
  \int\sqrt{x^{2}-a^{2}}\,dx = \frac{x\sqrt{x^{2}-a^{2}}}{2} - \frac{a^{2}}{2}\ln(x+\sqrt{x^{2}-a^{2}}) \\
  \int x\sqrt{x^{2}-a^{2}}\,dx = \frac{(x^{2}-a^{2})^{\frac{3}{2}}}{3} \\
  \int\frac{\sqrt{x^{2}-a^{2}}}{x}\,dx = \sqrt{x^{2}-a^{2}} - a\sec^{-1}\abs{\frac{x}{a}} \\
\end{tabular}


\subsection{$\sqrt{a^{2}-x^{2}}$}

\begin{tabular}{@{}>{$}l<{$}@{}}
  \int\frac{1}{\sqrt{a^{2}-x^{2}}}\,dx = sin^{-1}{\frac{x}{a}} \\
  \int{\frac{x}{\sqrt{a^{2}-x^{2}}}}\,dx = -\sqrt{a^{2}-x^{2}} \\
  \int\frac{1}{x\sqrt{a^{2}-x^{2}}}\,dx = -\frac{1}{a}\ln(\frac{a+\sqrt{a^{2}-x^{2}}}{x}) \\
  \int\sqrt{a^{2}-x^{2}}\,dx = \frac{x\sqrt{a^{2}-x^{2}}}{2}+\frac{a^{2}}{2}\sin^{-1}{\frac{x}{a}} \\
  \int x\sqrt{a^{2}-x^{2}}\,dx = -\frac{x(a^{2}-x^{2})^{\frac{3}{2}}}{3} \\
  \int\frac{\sqrt{a^{2}-x^{2}}}{x}\,dx = \sqrt{a^{2}-x^{2}}-a\ln(\frac{a+\sqrt{a^{2}-x^{2}}}{x}) \\
\end{tabular}


\subsection{$ax^{2}+bx+c$}

\begin{tabular}{@{}>{$}l<{$}@{}}
  \int\frac{1}{ax^{2}+bx+c}\,dx =
  \begin{cases}
      \frac{2}{\sqrt{4ac-b^{2}}}\tan^{-1}\frac{2ax+b}{\sqrt{4ac-b^{2}}} \\
      \frac{1}{\sqrt{b^{2}-4ac}}\ln(\frac{2ax+b-\sqrt{b^{2}-4ac}}{2ax+b+\sqrt{b^{2}-4ac}})
  \end{cases} \\
  \int\frac{x}{ax^{2}+bx+c}\,dx = \frac{1}{2a}\ln(ax^{2}+bx+c) - \frac{b}{2a}\int\frac{1}{ax^{2}+bx+c}\,dx \\
  \int\frac{x^{m}}{ax^{2}+bx+c}\,dx = \frac{x^{m-1}}{a(m-1)}-\frac{c}{a}\int\frac{x^{m-2}}{ax^{2}+bx+c}\,dx -\frac{b}{a}\int\frac{x^{m-1}}{ax^{2}+bx+c}\,dx \\
  \int\frac{1}{x(ax^{2}+bx+c)}\,dx = \frac{1}{2c}\ln(\frac{x^{2}}{ax^{2}+bx+c})-\frac{b}{2c}\int\frac{1}{ax^{2}+bx+c}\,dx \\
  \int\frac{1}{x^{n}(ax^{2}+bx+c)}\,dx = -\frac{1}{c(n-1)x^{n-1}}-\frac{b}{c}\int\frac{1}{x^{n-1}(ax^{2}+bx+c)}\,dx -\frac{a}{c}\int{1}{x^{n-2}(ax^{2}+bx+c)}\,dx \\
  \int\frac{x^{m}}{(ax^{2}+bx+c)^{n}}\,dx = -\frac{x^{m-1}}{a(2n-m-1)(ax^{2}+bx+c)^{n-1}}+\frac{c(m-1)}{a(2n-m-1)}\int\frac{x^{m-2}}{(ax^{2}+bx+c)^{n}} - \frac{b(n-m)}{a(2n-m-1)}\int\frac{x^{m-1}}{(ax^{2}+bx+c)^{n}}\,dx \\
  \int\frac{1}{x^{m}(ax^{2}+bx+c)^{n}} = -\frac{1}{c(m-1)x^{n-1}(ax^{2}+bx+c)^{n-1}}-\frac{a(m+2n-3)}{c(m-1)}\int\frac{1}{x^{m-2}(ax^{2}+bx+c)^{n}}\,dx - \frac{b(m+n-2)}{c(m-1)}\int\frac{1}{x^{m-1}(ax^{2}+bx+c)^{n-1}}\,dx
\end{tabular}



\subsection{$\sqrt{ax^{2}+bx+c}$}

\begin{tabular}{@{}>{$}l<{$}@{}}
  \int\frac{1}{\sqrt{ax^{2}+bx+c}} =
  \begin{cases}
      \frac{1}{\sqrt{a}}\ln(2\sqrt{a}\sqrt{ax^{2}+bx+c}+2ax+b) \\
      -\frac{1}{\sqrt{-a}}\sin^{-1}(\frac{2ax+b}{\sqrt{b^{2}-4ac}}) = \frac{1}{\sqrt{a}}\sinh^{-1}(\frac{2ax+b}{\sqrt{4ac-b^{2}}})
  \end{cases} \\
  \int\frac{x}{\sqrt{ax^{2}+bx+c}}\,dx = \frac{\sqrt{ax^{2}+bx+c}}{a}-\frac{b}{2a}\int\frac{1}{\sqrt{ax^{2}+bx+c}}\,dx \\
  \int\frac{1}{x\sqrt{ax^{2}+bx+c}}\,dx =
    \begin{cases}
      -\frac{1}{\sqrt{c}}\ln(\frac{2\sqrt{c}\sqrt{ax^{2}+bx+c}+bx+2c}{x}) \\
      \frac{1}{\sqrt{-c}}\sin^{-1}(\frac{bx+2c}{\abs{x}\sqrt{b^{2}-4ac}}) = -\frac{1}{\sqrt{c}}\sinh^{-1}(\frac{bx+2c}{\abs{x}\sqrt{4ac-b^{2}}})
    \end{cases} \\
    \int\sqrt{ax^{2}+bx+c}\,dx = \frac{(2ax+b)\sqrt{ax^{2}+bx+c}}{4a}+\frac{4ac-b^{2}}{8a}\int\frac{1}{\sqrt{ax^{2}+bx+c}}\,dx \\
    \int x\sqrt{ax^{2}+bx+c}\,dx = \frac{\sqrt{ax^{2}+bx+c})^{\frac{3}{2}}}{3a}-\frac{b(2ax+b)}{8a^{2}}\sqrt{ax^{2}+bx+c}  -\frac{b(4ac-b^{2})}{16a^{2}}\int\frac{1}{\sqrt{ax^{2}+bx+c}}\,dx \\
    \int\frac{\sqrt{ax^{2}+bx+c}}{x}\,dx = \sqrt{ax^{2}+bx+c}+\frac{b}{2}\int\frac{1}{\sqrt{ax^{2}+bx+c}}\,dx + c\int\frac{1}{x\sqrt{ax^{2}+bx+c}}\,dx \\
    \int(ax^{2}+bx+c)^{n+\frac{1}{2}}\,dx = \frac{(2ax+b)(ax^{2}+bx+c)^{n+\frac{1}{2}}}{4a(n+1)}+\frac{(2n+1)(4ac-b^{2})}{8a(n+1)}\int(ax^{2}+bx+c)^{n-\frac{1}{2}}\,dx \\
    \int x(ax^{2}+bx+c)^{n+\frac{1}{2}}\,dx = \frac{(ax^{2}+bx+c)^{n+\frac{3}{2}}}{a(2n+3)}-\frac{b}{2a}\int(ax^{2}+bx+c)^{n+\frac{1}{2}}\,dx \\
    \int\frac{1}{(ax^{2}+bx+c)^{n+\frac{1}{2}}}\,dx = \frac{2(2ax+b)}{(2n-1)(4ac-b^{2})(ax^{2}+bx+c)^{n-\frac{1}{2}}}+\frac{8a(n-1)}{(2n-1)(4ac-b^{2})}\int\frac{1}{(ax^{2}+bx+c)^{n-\frac{1}{2}}} \\
    \int\frac{1}{x(ax^{2}+bx+c)^{n+\frac{1}{2}}}\,dx = \frac{1}{c(2n-1)(ax^{2}+bx+c)^{n-\frac{1}{2}}}+\frac{1}{c}\int\frac{1}{x(ax^{2}+bx+c)^{n-\frac{1}{2}}}\,dx -\frac{b}{2c}\int\frac{1}{(ax^{2}+bx+c)^{n+\frac{1}{2}}}\,dx
  \end{tabular}



\subsection{$e^{ax}$}
  \begin{tabular}{@{}>{$}l<{$}@{}}
      \int e^{ax} \,d x = \frac{e^{ax}}{a} \\
      \int xe^{ax} \,d x = \frac{e^{ax}}{a} (x-frac{1}{a}) \\
      \int x^{n}e^{ax} \,dx = \frac{x^{n}e^{ax}}{a}-\frac{n}{a}\int x^{n-1}e^{ax}\,dx = \frac{e^{ax}}{a}(x^{n}-\frac{nx^{n-1}}{a}+\frac{n(n-1)x^{n-2}}{a^{2}}-\cdots\frac{(-1)^{n}n!}{a^{n}}) \\
      \int \frac{e^{ax}}{x}\,dx = \ln x + \frac{ax}{1\cdot 1!}+\frac{(ax)^{2}}{2\cdot 2!}+\frac{(ax)^{3}}{3\cdot 3!}+\cdots
  \end{tabular}
